Rewrote to get rid of foralls, stuck in fold_left proof

bloom-filter/Proof.BloomFilter.fst
@@ -14,230 +14,151 @@ open BloomFilter
 
 (**** Adjust slot properties ****)
 
-let modified_only_one_slot (old_bf:bloom_storage_u8) (new_bf:bloom_storage_u8) (idx:valid_index) =
-  forall (idx':valid_index{idx <> idx'}). slot_value new_bf idx' = slot_value old_bf idx'
+#reset-options "--max_fuel 0"
+
+let is_max (bf:bloom_storage_u8) (idx:valid_index) : Tot bool =
+ slot_value bf idx = U8.uint_to_t _MAX_U8
+
+let is_almost_max (bf:bloom_storage_u8) (idx:valid_index) : Tot bool =
+  slot_value bf idx = U8.(uint_to_t _MAX_U8 -^ 1uy)
 
 let adjust_slot_lemma (bf:bloom_storage_u8) (idx:valid_index)
-  (increment:bool) : Lemma (ensures (
+  (increment:bool) (idx':valid_index): Lemma (ensures (
     let new_bf = adjust_slot bf idx increment in
-    modified_only_one_slot bf new_bf idx /\
-    begin if increment then not (slot_is_empty new_bf idx) else true end
+    if idx' <> idx then
+      slot_value new_bf idx' = slot_value bf idx'
+    else begin
+      if is_max bf idx then
+        is_max new_bf idx
+      else if increment then
+	slot_value new_bf idx = U8.(slot_value bf idx +^ 1uy)
+      else if slot_is_empty bf idx then
+        is_max new_bf idx
+      else
+        slot_value new_bf idx = U8.(slot_value bf idx -^ 1uy)
+    end
   )) = ()
-
-let adjust_first_slot_lemma (bf:bloom_storage_u8) (hash:u32)
-  (increment:bool) : Lemma (ensures (
-    let new_bf = adjust_first_slot bf hash increment in
-    let idx = first_slot_index hash in
-    modified_only_one_slot bf new_bf idx /\
-    begin if increment then not (slot_is_empty new_bf idx) else true end
-  )) = adjust_slot_lemma bf (first_slot_index hash) increment
-
-let adjust_second_slot_lemma (bf:bloom_storage_u8) (hash:u32)
-  (increment:bool) : Lemma (ensures (
-    let new_bf = adjust_second_slot bf hash increment in
-    let idx = second_slot_index hash in
-    modified_only_one_slot bf new_bf idx /\
-    begin if increment then not (slot_is_empty new_bf idx) else true end
-  )) = adjust_slot_lemma bf (second_slot_index hash) increment
-
 
 (**** Insert hash properties ****)
 
-let modified_hash_slots (old_bf:bloom_storage_u8) (new_bf:bloom_storage_u8) (hash:u32) =
-  let idx1 = first_slot_index hash in
-  let idx2 = second_slot_index hash in
-  forall (idx':valid_index{idx' <> idx1 /\ idx' <> idx2}).
-  slot_value new_bf idx' = slot_value old_bf idx'
+let increase_or_saturate (old_bf:bloom_storage_u8) (new_bf:bloom_storage_u8)
+  (hash:u32) (idx:valid_index) =
+  let idx1 = first_slot_index hash in let idx2 = second_slot_index hash in
+  if is_max old_bf idx then
+    is_max new_bf idx
+  else if idx1 <> idx2 then
+    if idx = idx1 || idx = idx2 then
+      slot_value new_bf idx = U8.(slot_value old_bf idx +^ 1uy)
+    else slot_value new_bf idx = slot_value old_bf idx
+  else if idx = idx1 then
+      if is_almost_max old_bf idx1 then is_max new_bf idx1
+      else slot_value new_bf idx = U8.(slot_value old_bf idx +^ 2uy)
+  else slot_value new_bf idx = slot_value old_bf idx
 
-let insert_hash_prelim_lemma (bf: bloom_storage_u8) (idx: valid_index)
-  : Lemma (requires (U8.v (slot_value bf idx) < _MAX_U8))
-    (ensures (U8.v (slot_value (adjust_slot bf idx true) idx) = U8.v (slot_value bf idx) + 1))
+let insert_hash_lemma (old_bf: bloom_storage_u8) (hash:u32) (idx:valid_index)
+  : Lemma (ensures (
+    let idx1 = first_slot_index hash in let idx2 = second_slot_index hash in
+    let new_bf = insert_hash old_bf hash in
+    increase_or_saturate old_bf new_bf hash idx /\
+    might_contain_hash new_bf hash
+  ))
   = ()
-
-let increase_or_saturate (old_bf:bloom_storage_u8) (new_bf:bloom_storage_u8) (idx:valid_index) =
-  if U8.v (slot_value old_bf idx) = _MAX_U8 then
-    U8.v (slot_value new_bf idx) = _MAX_U8
-  else
-    U8.(slot_value new_bf idx >^ slot_value old_bf idx)
-
-let insert_hash_lemma1 (bf: bloom_storage_u8) (hash:u32)
-  : Lemma (ensures (increase_or_saturate bf (insert_hash bf hash) (first_slot_index hash)))
-  = let idx1 = first_slot_index hash in let idx2 = second_slot_index hash in
-  let bf0 = adjust_first_slot bf hash true in
-  adjust_first_slot_lemma bf hash true; adjust_second_slot_lemma bf0 hash true;
-  if U8.v (slot_value bf idx1) = _MAX_U8 then () else begin
-    insert_hash_prelim_lemma bf idx1;
-    if idx1 = idx2 then if U8.v (slot_value bf0 idx1) = _MAX_U8 then () else
-        insert_hash_prelim_lemma bf0 idx1
-    else ()
-  end
-
-let insert_hash_lemma2 (bf: bloom_storage_u8) (hash:u32)
-  : Lemma (ensures (increase_or_saturate bf (insert_hash bf hash) (second_slot_index hash)))
-  = let idx1 = first_slot_index hash in let idx2 = second_slot_index hash in
-  let bf0 = adjust_first_slot bf hash true in
-  adjust_first_slot_lemma bf hash true; adjust_second_slot_lemma bf0 hash true;
-  if U8.v (slot_value bf idx2) = _MAX_U8 then () else begin
-    insert_hash_prelim_lemma bf idx2;
-    if U8.v (slot_value bf0 idx2) = _MAX_U8 then () else
-        insert_hash_prelim_lemma bf0 idx2
-  end
-
-let insert_hash_lemma (bf:bloom_storage_u8) (hash:u32) : Lemma (ensures (
-    let new_bf = insert_hash bf hash in
-    let idx1 = first_slot_index hash in
-    let idx2 = second_slot_index hash in
-    modified_hash_slots bf new_bf hash /\
-    might_contain_hash new_bf hash /\
-    increase_or_saturate bf new_bf idx1 /\
-    increase_or_saturate bf new_bf idx2
-  )) = adjust_first_slot_lemma bf hash true;
-  let bf0 = adjust_first_slot bf hash true in
-  adjust_second_slot_lemma bf0 hash true;
-  insert_hash_lemma1 bf hash;
-  insert_hash_lemma2 bf hash
 
 (**** Remove hash properties ****)
 
-let decrease_by
-  (decr:u8) (old_bf:bloom_storage_u8) (new_bf:bloom_storage_u8) (idx:valid_index) =
-      if U8.v (slot_value new_bf idx) = _MAX_U8 then
-      U8.v (slot_value new_bf idx) = _MAX_U8
-    else if U8.(slot_value old_bf idx <^ decr) then
-      U8.v (slot_value new_bf idx) = _MAX_U8
-    else
-      slot_value new_bf idx = U8.(slot_value old_bf idx -^ decr)
+let is_almost_min (bf:bloom_storage_u8) (idx:valid_index) : Tot bool =
+  slot_value bf idx = 1uy
 
-let decrease_or_saturate
-  (old_bf:bloom_storage_u8) (new_bf:bloom_storage_u8) (idx1 idx2:valid_index)
-  =
-  if idx1 = idx2 then decrease_by 2uy old_bf new_bf idx1 else
-    decrease_by 1uy old_bf new_bf idx1 && decrease_by 1uy old_bf new_bf idx2
+let decrease_or_saturate (old_bf:bloom_storage_u8) (new_bf:bloom_storage_u8)
+  (hash:u32) (idx:valid_index) =
+  let idx1 = first_slot_index hash in let idx2 = second_slot_index hash in
+  if is_max old_bf idx then
+    is_max new_bf idx
+  else if idx1 <> idx2 then
+    if idx = idx1 || idx = idx2 then
+      if slot_is_empty old_bf idx then
+        is_max new_bf idx
+      else
+        slot_value new_bf idx = U8.(slot_value old_bf idx -^ 1uy)
+    else slot_value new_bf idx = slot_value old_bf idx
+  else if idx = idx1 then
+      if is_almost_min old_bf idx || slot_is_empty old_bf idx then is_max new_bf idx
+      else slot_value new_bf idx = U8.(slot_value old_bf idx -^ 2uy)
+  else slot_value new_bf idx = slot_value old_bf idx
 
-let underflow_lemma () : Lemma (ensures (U8.(v (0uy -%^ 1uy)) = _MAX_U8)) =
-  assert_norm(U8.(v (0uy -%^ 1uy)) = _MAX_U8)
-
-let remove_hash_prelim_lemma (bf:bloom_storage_u8) (idx:valid_index)
-  : Lemma (ensures (decrease_by 1uy bf (adjust_slot bf idx false) idx)) =
-  ()
-
-let remove_hash_lemma (bf: bloom_storage_u8) (hash:u32)
+let remove_hash_lemma (bf: bloom_storage_u8) (hash:u32) (idx:valid_index)
   : Lemma (ensures (
     let new_bf = remove_hash bf hash in
     let idx1 = first_slot_index hash in
     let idx2 = second_slot_index hash in
-    decrease_or_saturate bf new_bf idx1 idx2
+    decrease_or_saturate bf new_bf hash idx
    ))
-  = underflow_lemma ();
-  let idx1 = first_slot_index hash in let idx2 = second_slot_index hash in
-  remove_hash_prelim_lemma bf idx1;
-  let bf0 = adjust_slot bf idx1 false in
-  remove_hash_prelim_lemma bf0 idx2
+  = ()
 
 (**** Insert element properties ****)
 
-let element_invalidation (bf: bloom_storage_u8) =
-  (forall (e:element). (
-    (not (might_contain_hash bf (hash e))) ==>
-      (not (contains bf.ghost_state.elements e))
-  ))
+let element_invalidation (bf: bloom_storage_u8) (e:element) =
+  not (might_contain_hash bf (hash e)) ==> not (contains bf.ghost_state.elements e)
+
+let one_element_count (idx:valid_index) (sum: count) (e_count: (element & count)) : Tot count =
+   let (e, count) = e_count in
+   let sum = if first_slot_index (hash e) = idx then sum + count else sum in
+   if second_slot_index (hash e) = idx then sum + count else sum
 
 let all_elements_counts (bf:bloom_storage_u8) (idx:valid_index) : Tot count =
-   List.Tot.Base.fold_left (fun (sum : count) ((e, count) : (element & count)) ->
-     let sum = if first_slot_index (hash e) = idx then sum + count else sum in
-     if second_slot_index (hash e) = idx then sum + count else sum
-   ) 0 bf.ghost_state.elements
+   List.Tot.Base.fold_left (one_element_count idx) 0 bf.ghost_state.elements
 
-let count_invariant_property (bf:bloom_storage_u8) (e:element) : Tot bool =
-  let hash_e = hash e in
-  let idx1 = first_slot_index hash_e in let idx2 = second_slot_index hash_e in
-  let val1 = slot_value bf idx1 in let val2 = slot_value bf idx2 in
-  begin if U8.v val1 = _MAX_U8 then true else
-    all_elements_counts bf idx1 = U8.v val1
-  end && begin if U8.v val2 = _MAX_U8 then true else
-    all_elements_counts bf idx2 = U8.v val2
-  end
+let count_invariant_property (bf:bloom_storage_u8) (idx:valid_index) : Tot bool =
+  if is_max bf idx then true else
+    all_elements_counts bf idx = U8.v (slot_value bf idx)
 
-let count_invariant (bf:bloom_storage_u8) =
-   (forall (e:element{contains bf.ghost_state.elements e}).
-    count_invariant_property bf e)
+let count_invariant (bf:bloom_storage_u8) (idx:valid_index) =
+    count_invariant_property bf idx
 
-let valid_bf (bf:bloom_storage_u8) = element_invalidation bf /\ count_invariant bf
+let insert_element_element_invalidation_lemma (bf:bloom_storage_u8) (e:element) (e':element)
+  : Lemma (requires (element_invalidation bf e'))
+    (ensures (element_invalidation (insert_element bf e) e'))
+  = ()
 
+#reset-options "--max_fuel 2"
 
-let insert_element_lemma_count_invariant_prelim (bf:bloom_storage_u8) (e:element) (idx:valid_index)
-  : Lemma (requires (all_elements_counts bf idx = U8.v (slot_value bf idx))) (ensures (
-    let new_bf = insert_hash bf (hash e) in
-    if U8.v (slot_value new_bf idx) = _MAX_U8 then true else
-      all_elements_counts new_bf idx = U8.v (slot_value new_bf idx)
-  )) = insert_hash_lemma bf (hash e);admit()
+let insert_element_all_elements_counts_lemma1 (bf:bloom_storage_u8) (e:element)
+  : Lemma (requires (first_slot_index (hash e) <> second_slot_index (hash e)))
+    (ensures (let new_bf = insert_element bf e in
+       let idx1 = first_slot_index (hash e) in let idx2 = second_slot_index (hash e) in
+       all_elements_counts new_bf idx1 = all_elements_counts bf idx1 + 1 &&
+       all_elements_counts new_bf idx2 = all_elements_counts bf idx2 + 1
+    ))
+  = admit()
 
-let insert_element_lemma_count_invariant (bf:bloom_storage_u8) (e:element)
-  : Lemma (requires (valid_bf bf)) (ensures (valid_bf (insert_element bf e)))
-  = let hash_e = hash e in let new_bf = insert_hash bf hash_e in
-  insert_hash_lemma bf (hash e);
-  let forall_intro_lemma (e':element{contains new_bf.ghost_state.elements e'})
-    : Lemma (ensures (count_invariant_property new_bf e')) =
-    assert(count_invariant_property bf e');
-    let hash_e' = hash e' in
-    let idx1_e' = first_slot_index hash_e' in let idx2_e' = second_slot_index hash_e' in
-    begin if U8.v (slot_value bf idx1_e') = _MAX_U8 then
-      assert(U8.v (slot_value new_bf idx1_e') = _MAX_U8)
-    else
-      insert_element_lemma_count_invariant_prelim bf e idx1_e'
-    end;
-     begin if U8.v (slot_value bf idx2_e') = _MAX_U8 then
-      assert(U8.v (slot_value new_bf idx2_e') = _MAX_U8)
-    else
-      insert_element_lemma_count_invariant_prelim bf e idx2_e'
-    end
-  in Classical.forall_intro forall_intro_lemma
+let insert_element_all_elements_counts_lemma2 (bf:bloom_storage_u8) (e:element)
+  : Lemma (requires (first_slot_index (hash e) = second_slot_index (hash e)))
+    (ensures (let new_bf = insert_element bf e in
+       let idx = first_slot_index (hash e) in
+       all_elements_counts new_bf idx = all_elements_counts bf idx + 2
+    ))
+  = admit()
+
+#reset-options "--max_fuel 0"
+
+let insert_element_count_invariant_lemma
+  (bf:bloom_storage_u8) (e:element) (idx:valid_index)
+  : Lemma (requires (not (is_max bf idx) /\ all_elements_counts bf idx = U8.v (slot_value bf idx)))
+    (ensures (let new_bf = insert_element bf e in
+      not (is_max new_bf idx) ==> all_elements_counts new_bf idx = U8.v (slot_value new_bf idx)
+    ))
+  = insert_hash_lemma bf (hash e) idx;
+  let idx1 = first_slot_index (hash e) in let idx2 = second_slot_index (hash e) in
+  let new_bf = insert_element bf e in
+  if idx1 <> idx2 then
+    if idx = idx1 || idx = idx2 then
+      if is_max new_bf idx then () else insert_element_all_elements_counts_lemma1 bf e
+    else ()
+  else if idx = idx1 then
+      if is_almost_max bf idx1 then ()
+      else insert_element_all_elements_counts_lemma2 bf e
+  else ()
 
 (**** Remove element properties ****)
 
-let lemma1 (bf:bloom_storage_u8) (hash:u32) (idx:valid_index)
-  : Lemma (requires (U8.(slot_value bf idx >^ 2uy)))
-  (ensures (let new_bf = remove_hash bf hash in
-    U8.(slot_value new_bf idx >^ 0uy)
-  )) = remove_hash_lemma bf hash
-
-let lemma2 (bf:bloom_storage_u8) (hash:u32) (idx:valid_index)
-  : Lemma (requires (
-    U8.(slot_value bf idx >^ 1uy) /\ first_slot_index hash <> second_slot_index hash
-  )) (ensures (let new_bf = remove_hash bf hash in
-    U8.(slot_value new_bf idx >^ 0uy)
-  )) = remove_hash_lemma bf hash
-
-let lemma3 (n:nat) : Lemma (requires (n <= 2 /\ n > 1)) (ensures (n = 2)) = ()
-
-#reset-options "--z3rlimit 10"
-
-let remove_element_lemma_element_invalidation
-  (bf:bloom_storage_u8) (e:element{contains bf.ghost_state.elements e})
-  : Lemma(requires (valid_bf bf)) (ensures (element_invalidation (remove_element bf e))) =
-  let new_bf = remove_element bf e in let hash_e = hash e in
-  let idx1_e = first_slot_index hash_e in let idx2_e = second_slot_index hash_e in
-  let forall_intro_lemma (e':element{contains new_bf.ghost_state.elements e'})
-    : Lemma (ensures (might_contain_hash new_bf (hash e'))) =
-    let hash_e' = hash e' in if e <> e' then begin
-      let idx1_e' = first_slot_index hash_e' in let idx2_e' = second_slot_index hash_e' in
-      assert(contains bf.ghost_state.elements e');
-      assert(might_contain_hash bf hash_e');
-      assert(count_invariant_property bf e');
-      let e'_count =  element_count bf.ghost_state.elements e' in
-      if e'_count > 2 then begin
-	lemma1 bf hash_e idx1_e';lemma1 bf hash_e idx2_e'
-      end else if e'_count > 1 then
-	if idx1_e = idx2_e then begin
-	  lemma3 e'_count;assert(e'_count = 2);admit()
-	end else (lemma2 bf hash_e idx1_e';lemma2 bf hash_e idx2_e')
-      else begin
-        //assert(e'_count = 1);
-        admit()
-      end
-    end else begin
-      assert(e = e');
-      admit()
-    end
-  in
-  Classical.forall_intro forall_intro_lemma
+let _ = ()
